src/promising/TsoPromising2.v
@@ -1020,133 +1020,11 @@ Module Machine.
       ss. congr.
   Qed.
 
-  Definition promises_from_mem
-             (tid:Id.t) (mem: Memory.t): Promises.t.
-  Proof.
-    induction mem using list_rev_rect.
-    - exact bot.
-    - destruct x.
-      apply (if tid0 == tid
-             then Promises.set (S (List.length (List.rev mem0))) IHmem
-             else IHmem).
-  Defined.
-
-  Lemma promises_from_mem_nil tid:
-    promises_from_mem tid Memory.empty = bot.
-  Proof.
-    unfold promises_from_mem, list_rev_rect, eq_rect. ss.
-    match goal with
-    | [|- context[match ?c with | eq_refl => _ end]] => destruct c
-    end; ss.
-  Qed.
-
-  Lemma promises_from_mem_snoc tid mem msg:
-    promises_from_mem tid (mem ++ [msg]) =
-    if msg.(Msg.tid) == tid
-    then Promises.set (S (List.length mem)) (promises_from_mem tid mem)
-    else promises_from_mem tid mem.
-  Proof.
-    unfold promises_from_mem at 1, list_rev_rect, eq_rect.
-    match goal with
-    | [|- context[match ?c with | eq_refl => _ end]] => destruct c
-    end; ss.
-    rewrite List.rev_involutive, List.rev_app_distr. ss.
-    destruct msg. s. condtac.
-    - inversion e. subst. rewrite ? List.rev_length.
-      f_equal.
-      unfold promises_from_mem, list_rev_rect, eq_rect.
-      match goal with
-      | [|- context[match ?c with | eq_refl => _ end]] => destruct c
-      end; ss.
-    - unfold promises_from_mem, list_rev_rect, eq_rect.
-      match goal with
-      | [|- context[match ?c with | eq_refl => _ end]] => destruct c
-      end; ss.
-  Qed.
-
-  Lemma promises_from_mem_inv
-        ts tid mem
-        (LOOKUP: Promises.lookup (S ts) (promises_from_mem tid mem)):
-    exists loc val, List.nth_error mem ts = Some (Msg.mk loc val tid).
-  Proof.
-    revert LOOKUP. induction mem using List.rev_ind.
-    { rewrite promises_from_mem_nil, Promises.lookup_bot. ss. }
-    rewrite promises_from_mem_snoc. condtac.
-    { rewrite Promises.set_o. condtac.
-      - inversion e. inversion e0. subst.
-        rewrite List.nth_error_app2; [|lia].
-        rewrite Nat.sub_diag. ss.
-        destruct x. esplits; eauto.
-      - i. exploit IHmem; eauto.  i. des.
-        rewrite List.nth_error_app1; eauto.
-        apply List.nth_error_Some. congr.
-    }
-    i. exploit IHmem; eauto.  i. des.
-    rewrite List.nth_error_app1; eauto.
-    apply List.nth_error_Some. congr.
-  Qed.
-
-  Lemma promises_from_mem_lookup
-        mem ts loc val tid
-        (GET: List.nth_error mem ts = Some (Msg.mk loc val tid)):
-    Promises.lookup (S ts) (promises_from_mem tid mem).
-  Proof.
-    revert GET. induction mem using List.rev_ind.
-    { i. apply List.nth_error_In in GET. inv GET. }
-    rewrite promises_from_mem_snoc. condtac.
-    - rewrite Promises.set_o. condtac.
-      + inversion e. inversion e0. subst.
-        rewrite List.nth_error_app2; [|lia].
-        rewrite Nat.sub_diag. ss.
-      + i. apply IHmem.
-        erewrite <- List.nth_error_app1; eauto.
-        assert (H: ts < List.length (mem0 ++ [x])).
-        { rewrite <- List.nth_error_Some. ii. congr. }
-        rewrite List.app_length in H.
-        rewrite Nat.add_1_r in H. inv H; try lia.
-        exfalso. apply c. ss.
-    - i. apply IHmem.
-      destruct (Nat.eq_dec ts (List.length mem0)) eqn:Heq.
-      + inv Heq. rewrite List.nth_error_app2 in GET; try lia.
-        rewrite Nat.sub_diag in GET. ss. inv GET. ss.
-        exfalso. apply c. ss.
-      + rewrite List.nth_error_app1 in GET; auto.
-        assert (H: ts < List.length (mem0 ++ [x])).
-        { rewrite <- List.nth_error_Some. ii. congr. }
-        rewrite List.app_length in H.
-        rewrite Nat.add_1_r in H. inv H; try lia; congr.
-  Qed.
-
-  Lemma promises_from_mem_spec
-        ts tid mem:
-    Promises.lookup (S ts) (promises_from_mem tid mem) <->
-    exists loc val, List.nth_error mem ts = Some (Msg.mk loc val tid).
-  Proof.
-    induction mem using List.rev_ind.
-    { econs.
-      - rewrite promises_from_mem_nil, Promises.lookup_bot. ss.
-      - i. des. destruct ts; ss.
-    }
-    rewrite promises_from_mem_snoc. econs.
-    - condtac.
-      + inversion e. subst. rewrite Promises.set_o. condtac.
-        * inversion e0. subst. i.
-          rewrite List.nth_error_app2, Nat.sub_diag; [|lia]. ss.
-          destruct x. ss. eauto.
-        * intro Y. apply IHmem in Y. des.
-          esplits; eauto. apply nth_error_app_mon. eauto.
-      + intro Y. apply IHmem in Y. des.
-        esplits; eauto. apply nth_error_app_mon. eauto.
-    - i. des. apply nth_error_snoc_inv in H. des; ss.
-      { condtac; eauto. rewrite Promises.set_o. condtac; eauto. }
-      subst. condtac; ss; [|congr]. rewrite Promises.set_o. condtac; [|congr]. ss.
-  Qed.
-
   Definition init_with_promises (p:program) (mem:Memory.t): Machine.t :=
     Machine.mk
       (IdMap.mapi (fun tid stmts =>
                      (State.init stmts,
-                      Local.init_with_promises (promises_from_mem tid mem)))
+                      Local.init_with_promises (Promises.promises_from_mem tid mem)))
                   p)
       mem.
 
@@ -1162,7 +1040,7 @@ Module Machine.
     { esplits; eauto. ii. s. rewrite IdMap.map_spec, IdMap.mapi_spec.
       destruct (IdMap.find y p); ss.
       unfold Local.init, Local.init_with_promises. repeat f_equal.
-      rewrite promises_from_mem_nil. ss.
+      rewrite Promises.promises_from_mem_nil. ss.
     }
     exploit IHpromises; eauto.
     { i. apply MEM. apply List.in_app_iff. intuition. }
@@ -1182,9 +1060,9 @@ Module Machine.
     - s. ii. rewrite IdMap.add_spec. condtac; ss.
       + inversion e. subst. rewrite IdMap.mapi_spec, FIND. s.
         unfold Local.init_with_promises. repeat f_equal.
-        rewrite promises_from_mem_snoc. condtac; ss.
+        rewrite Promises.promises_from_mem_snoc. condtac; ss.
       + rewrite TPOOL, ? IdMap.mapi_spec. destruct (IdMap.find y p); ss.
-        unfold Local.init_with_promises. rewrite promises_from_mem_snoc. s.
+        unfold Local.init_with_promises. rewrite Promises.promises_from_mem_snoc. s.
         condtac; ss. congr.
     - ss.
   Qed.
@@ -1199,13 +1077,13 @@ Module Machine.
     induction STEP.
     { s. ii. rewrite IdMap.map_spec, IdMap.mapi_spec.
       destruct (IdMap.find y p); ss. f_equal. f_equal.
-      rewrite promises_from_mem_nil. ss.
+      rewrite Promises.promises_from_mem_nil. ss.
     }
     destruct y as [tpool2 mem2].
     destruct z as [tpool3 mem3].
     ss. inv H. inv STEP0. inv LOCAL. ss. subst. inv MEM2.
     ii. generalize (IHSTEP y). rewrite IdMap.add_spec, ? IdMap.mapi_spec.
-    rewrite promises_from_mem_snoc. s.
+    rewrite Promises.promises_from_mem_snoc. s.
     repeat condtac; try congr.
     inversion e. subst. rewrite FIND. destruct (IdMap.find tid p); ss. i. inv H. ss.
   Qed.
