src/axiomatic/TsoPFtoA1.v
@@ -617,7 +617,7 @@ Proof.
   { i. simplify. ss. econs; ss.
     - rewrite IdMap.mapi_spec, STMT in FIND. inv FIND. s. i.
       left. splits; ss. destruct ts; ss.
-      eapply Machine.promises_from_mem_lookup. eauto.
+      eapply Promises.promises_from_mem_lookup. eauto.
     - i. des. destruct eid; ss.
     - i. des. destruct eid; ss.
     - i. des. destruct eid; ss.
@@ -629,11 +629,11 @@ Proof.
       econs; ss; i; try by apply bot_spec.
       + econs; esplits; ss.
       + destruct ts; ss.
-        rewrite Machine.promises_from_mem_spec in IN. des.
+        rewrite Promises.promises_from_mem_spec in IN. des.
         apply lt_le_S. rewrite <- List.nth_error_Some. ii. congr.
       + destruct ts; ss.
         unfold Memory.get_msg in *. ss. destruct msg.
-        exploit Machine.promises_from_mem_lookup; eauto. ss. subst. ss.
+        exploit Promises.promises_from_mem_lookup; eauto. ss. subst. ss.
   }
   clear LOCAL.
   i. simplify.
